some proofs

theories/Codata/Simulation.v
@@ -1,13 +1,110 @@
 
 From Paco Require Import paco.
 
-Definition Chain (X Y : Type) := X -> Y -> forall P : Type, (P -> X) -> (P -> Y) -> Type.
+Definition ObRel (X Y : Type) := X -> Y -> forall P : Type, (P -> X) -> (P -> Y) -> Prop.
 
-Variant simulationF {X Y} (R : Chain X Y) vclo (sim : X -> Y -> Prop) : X -> Y -> Prop :=
+Variant simulationF {X Y} (R : ObRel X Y) (vclo : (X -> Y -> Prop) -> (X -> Y -> Prop)) (sim : X -> Y -> Prop) : X -> Y -> Prop :=
 | Step t1 t2 P k1 k2
        (REL : R t1 t2 P k1 k2)
        (RELS : forall p : P, vclo sim (k1 p) (k2 p))
   : simulationF R vclo sim t1 t2
 .
 
-Definition simulation {X Y} (R : Chain X Y) vclo := paco2 (simulationF R vclo).
+Definition simulation {X Y} (R : ObRel X Y) vclo := paco2 (simulationF R vclo) bot2.
+
+Lemma simulationF_mono {X Y} (R : ObRel X Y) vclo (MON : monotone2 vclo)
+  : monotone2 (simulationF R vclo).
+Proof.
+  unfold monotone2; intros.
+  destruct IN. econstructor; eauto.
+Qed.
+Hint Resolve simulationF_mono : paco.
+
+Definition flip_obrel {X Y} (R : ObRel X Y) : ObRel Y X :=
+  fun tx ty P kx ky => R ty tx P ky kx.
+
+Definition flip_clo {A B C} clo r := @flip A B C (clo (@flip B A C r)).
+
+Lemma flip_clo_mono {X Y} (vclo : (X -> Y -> Prop) -> X -> Y -> Prop)
+  : monotone2 vclo -> monotone2 (flip_clo vclo).
+Proof. compute; firstorder. Qed.
+Hint Resolve flip_clo_mono : paco.
+
+Lemma eqit_idclo_mono {X Y} : monotone2 (@id (X -> Y -> Prop)).
+Proof. unfold id. eauto. Qed.
+Hint Resolve eqit_idclo_mono : paco.
+
+Lemma simulation_flip {X Y} (R : ObRel X Y) vclo (MON : monotone2 vclo) :
+  forall (t1 : X) (t2 : Y),
+    simulation (flip_obrel R) (flip_clo vclo) t2 t1 -> simulation R vclo t1 t2.
+Proof.
+  pcofix CIH; pstep. intros t1 t2 H.
+  punfold H; destruct H.
+  econstructor; [ eapply REL | ].
+  intros; specialize (RELS p).
+  eapply MON; [ eapply RELS | ].
+  intros t1' t2' H'; pclearbot.
+  eauto.
+Qed.
+
+Lemma simulation_mono {X Y} (R R' : ObRel X Y) vclo
+      (MON : monotone2 vclo)
+      (LE : R <5= R') :
+  simulation R vclo <2= simulation R' vclo.
+Proof.
+  pcofix CIH; pstep. intros x y PR; punfold PR; destruct PR.
+  econstructor; [eauto|].
+  intros; eapply MON; [eapply RELS |].
+  intros; pclearbot; eauto.
+Qed.
+
+From Coq Require Import
+     RelationClasses.
+
+Lemma Reflexive_simulationF {X} (R : ObRel X X) vclo sim
+      (REFL_R : forall x, exists P k, R x x P k k)
+      (REFL_hom : forall R, Reflexive R -> Reflexive (vclo R))
+      (REFL_sim : Reflexive sim) :
+  Reflexive (simulationF R vclo sim).
+Proof.
+  unfold Reflexive; intros; specialize (REFL_R x).
+  destruct REFL_R as [ P [ k REFL ] ].
+  econstructor; [ eapply REFL | ].
+  intros; eapply REFL_hom; eauto.
+Qed.
+
+Lemma Reflexive_simulation {X} (R : ObRel X X) vclo
+      (MON : monotone2 vclo)
+      (REFL_R : forall x, exists P k, R x x P k k)
+      (REFL_hom : forall R, Reflexive R -> Reflexive (vclo R)) :
+  Reflexive (simulation R vclo).
+Proof.
+  unfold Reflexive; pcofix CIH; pstep.
+  intros x; destruct (REFL_R x) as [P [k REFL]].
+  econstructor; [eapply REFL|].
+  intros; eapply MON; [eapply REFL_hom; eauto |].
+  intros; eauto.
+Qed.
+
+Lemma Symmetric_simulationF {X} (R : ObRel X X) vclo sim
+      (SYM_R : forall x y P x' y', R x y P x' y' -> R y x P y' x')
+      (SYM_hom : forall R, Symmetric R -> Symmetric (vclo R))
+      (SYM_sim : Symmetric sim) :
+  Symmetric (simulationF R vclo sim).
+Proof.
+  unfold Symmetric. intros.
+  destruct H.
+  econstructor.
+  eapply SYM_R. eapply REL.
+  intros. eapply SYM_hom; eauto.
+Qed.
+
+Lemma Symmetric_simulation {X} (R : ObRel X X)
+      (SYM_R : forall x y P x' y', R x y P x' y' -> R y x P y' x') :
+  Symmetric (simulation R id).
+Proof.
+  pcofix CIH. pstep.
+  intros x y H. punfold H. destruct H. pclearbot.
+  econstructor; [eapply SYM_R; eapply REL|].
+  intros. right. eapply CIH. eapply RELS.
+Qed.
